added the construction of the cover(unfinished)

original_work/TS_To_XC/TS_To_XC.thy
@@ -12,37 +12,38 @@ definition literals_of_sat :: "'a three_sat \<Rightarrow> 'a xc_element set" whe
 "literals_of_sat F = comp_literals F {}"
 
 definition literal_sets
-  :: "'a xc_element set \<Rightarrow> 'a xc_element set set" where
-"literal_sets Li = {{l}| l. l \<in> Li}"
+  :: "'a three_sat  \<Rightarrow> 'a xc_element set set" where
+"literal_sets F = {{l}| l. l \<in> (literals_of_sat F)}"
 
 definition clauses_with_literals 
-  :: "'a xc_element set \<Rightarrow> 'a xc_element set \<Rightarrow> 'a xc_element set set" where
-"clauses_with_literals Cl Li = {{C c, l} |c l. C c \<in> Cl \<and> l \<in> Li 
+  :: "'a three_sat \<Rightarrow> 'a xc_element set set" where
+"clauses_with_literals F = {{C c, l} |c l. C c \<in> (clauses_of_sat F) \<and> l \<in> (literals_of_sat F) 
         \<and> l \<in> {L a c | a. a \<in> c}}"
 
 definition var_true_literals
-  :: "'a xc_element set \<Rightarrow> 'a xc_element set \<Rightarrow> 'a xc_element set 
-       \<Rightarrow> 'a xc_element set set" where 
-"var_true_literals Va Cl Li = 
-  {{V v} \<union> {l. l \<in> Li \<and> (\<exists>c. C c\<in> Cl \<and> L (Neg v) c = l)} |v. V v \<in> Va}"
+  :: "'a three_sat \<Rightarrow> 'a xc_element set set" where 
+"var_true_literals F = 
+  {{V v} \<union> {l. l \<in> (literals_of_sat F) 
+  \<and> (\<exists>c. C c\<in> (clauses_of_sat F) \<and> L (Neg v) c = l)} |v. V v \<in> (vars_of_sat F)}"
 
 definition var_false_literals
-  :: "'a xc_element set \<Rightarrow> 'a xc_element set \<Rightarrow> 'a xc_element set 
-       \<Rightarrow> 'a xc_element set set" where 
-"var_false_literals Va Cl Li = 
-  {{V v} \<union> {l. l \<in> Li \<and> (\<exists>c. C c\<in> Cl \<and> L (Pos v) c = l)} |v. V v \<in> Va}"
+    :: "'a three_sat \<Rightarrow> 'a xc_element set set" where 
+"var_false_literals F = 
+  {{V v} \<union> {l. l \<in> (literals_of_sat F) 
+  \<and> (\<exists>c. C c\<in> (clauses_of_sat F) \<and> L (Pos v) c = l)} |v. V v \<in> (vars_of_sat F)}"
 
 definition ts_xc :: "'a three_sat \<Rightarrow> 'a xc_element set * 'a xc_element set set" where 
 "ts_xc F =(let
    vars = vars_of_sat F;
    clauses = clauses_of_sat F;
    literals = literals_of_sat F;
-   literals_sets = literal_sets literals;
-   clause_with_literal_sets = clauses_with_literals clauses literals;
+   literals_sets = literal_sets F;
+   clause_with_literal_sets = 
+     clauses_with_literals F;
    var_true_sets = 
-    var_true_literals vars clauses literals;
+    var_true_literals F;
    var_false_sets = 
-    var_false_literals vars clauses literals
+    var_false_literals F
   in
    (vars \<union> clauses \<union> literals,
     literals_sets \<union> clause_with_literal_sets \<union> var_true_sets \<union> var_false_sets))"
@@ -55,10 +56,10 @@ proof -
   let ?clauses = "clauses_of_sat F"
   let ?literals = "literals_of_sat F"
 
-  let ?ls = "literal_sets ?literals"
-  let ?cs = "clauses_with_literals ?clauses ?literals"
-  let ?vt = "var_true_literals ?vars ?clauses ?literals"
-  let ?vf = "var_false_literals ?vars ?clauses ?literals"
+  let ?ls = "literal_sets F"
+  let ?cs = "clauses_with_literals F"
+  let ?vt = "var_true_literals F"
+  let ?vf = "var_false_literals F"
 
   have x_part: "X = ?vars \<union> ?clauses \<union> ?literals"
   using assms ts_xc_def[of F] by (auto simp: Let_def)
@@ -74,7 +75,7 @@ proof -
 
   moreover have "\<Union>?vt \<subseteq> ?literals \<union> ?vars"
     unfolding var_true_literals_def by blast
-    
+
   moreover have "\<Union>?vf \<subseteq> ?literals \<union> ?vars" 
     unfolding var_false_literals_def by blast
 
@@ -83,5 +84,21 @@ proof -
 
   with x_part s_part show ?thesis by force
 qed 
+
+definition constr_cover 
+  :: "'a three_sat \<Rightarrow> ('a \<Rightarrow> bool) \<Rightarrow> 'a xc_element set set" where 
+"constr_cover F \<sigma> \<equiv> 
+  (if F \<in> three_cnf_sat 
+  then 
+  (let
+     vars_sets = 
+       {x_set | x_set. \<exists>x \<in> vars F.
+       (if (\<sigma>\<up>) (Pos x) then (V x) \<in> x_set \<and> x_set \<in> var_true_literals F
+       else (V x) \<in> x_set \<and> x_set \<in> var_false_literals F)};
+     clause_sets = 
+       {{C c, p} | c p. c \<in> (set F) \<and> p \<in> c}
+   in 
+    S')
+  else {})"
 
 end
